[riscvpmp] split up model

case_study/RiscvPmp/Model.v
@@ -32,7 +32,7 @@ From Coq Require Import
 From Katamaran Require Import
      Bitvector
      Environment
-     Iris.Logic
+     Iris.Instance
      Iris.Model
      Program
      Semantics
@@ -41,6 +41,8 @@ From Katamaran Require Import
      Specification
      RiscvPmp.Machine
      RiscvPmp.Contracts
+     RiscvPmp.IrisModel
+     RiscvPmp.IrisInstance
      RiscvPmp.Sig.
 From Equations Require Import
      Equations.
@@ -54,11 +56,6 @@ From iris.proofmode Require Import string_ident tactics.
 
 Set Implicit Arguments.
 Import ListNotations.
-
-Module gh := iris.base_logic.lib.gen_heap.
-
-Module RiscvPmpSemantics <: Semantics RiscvPmpBase RiscvPmpProgram :=
-  MakeSemantics RiscvPmpBase RiscvPmpProgram.
 
 Import RiscvPmpProgram.
 Import RiscvPmpSignature.
@@ -75,171 +72,8 @@ Ltac destruct_syminstance ι :=
     | _ => idtac
     end.
 
-Module Import RiscvPmpIrisBase <: IrisBase RiscvPmpBase RiscvPmpProgram RiscvPmpSemantics.
-  Include IrisPrelims RiscvPmpBase RiscvPmpProgram RiscvPmpSemantics.
-
-  Section RiscvPmpIrisParams.
-    Import iris.bi.interface.
-    Import iris.bi.big_op.
-    Import iris.base_logic.lib.iprop.
-    Import iris.base_logic.lib.gen_heap.
-
-    Definition MemVal : Set := Word.
-
-    Class mcMemGS Σ :=
-      McMemGS {
-          (* ghost variable for tracking state of registers *)
-          mc_ghGS : gh.gen_heapGS Addr MemVal Σ
-        }.
-    #[export] Existing Instance mc_ghGS.
-
-    Definition memGpreS : gFunctors -> Set := fun Σ => gh.gen_heapGpreS Z MemVal Σ.
-    Definition memGS : gFunctors -> Set := mcMemGS.
-    Definition memΣ : gFunctors := gh.gen_heapΣ Addr MemVal.
-
-    Definition liveAddrs := seqZ minAddr (maxAddr - minAddr + 1).
-    Definition initMemMap μ := (list_to_map (map (fun a => (a , μ a)) liveAddrs) : gmap Addr MemVal).
-
-    Definition memΣ_GpreS : forall {Σ}, subG memΣ Σ -> memGpreS Σ :=
-      fun {Σ} => gh.subG_gen_heapGpreS (Σ := Σ) (L := Addr) (V := MemVal).
-
-    Definition mem_inv : forall {Σ}, mcMemGS Σ -> Memory -> iProp Σ :=
-      fun {Σ} hG μ =>
-        (∃ memmap, gen_heap_interp memmap ∗
-           ⌜ map_Forall (fun a v => μ a = v) memmap ⌝
-        )%I.
-
-    Definition mem_res : forall {Σ}, mcMemGS Σ -> Memory -> iProp Σ :=
-      fun {Σ} hG μ =>
-        ([∗ map] l↦v ∈ initMemMap μ, mapsto l (DfracOwn 1) v) %I.
-
-    Lemma initMemMap_works μ : map_Forall (λ (a : Addr) (v : MemVal), μ a = v) (initMemMap μ).
-    Proof.
-      unfold initMemMap.
-      rewrite map_Forall_to_list.
-      rewrite Forall_forall.
-      intros (a , v).
-      rewrite elem_of_map_to_list.
-      intros el.
-      apply elem_of_list_to_map_2 in el.
-      apply elem_of_list_In in el.
-      apply in_map_iff in el.
-      by destruct el as (a' & <- & _).
-    Qed.
-
-    Lemma mem_inv_init : forall Σ (μ : Memory), memGpreS Σ ->
-      ⊢ |==> ∃ mG : mcMemGS Σ, (mem_inv mG μ ∗ mem_res mG μ)%I.
-    Proof.
-      iIntros (Σ μ gHP).
-
-      iMod (gen_heap_init (gen_heapGpreS0 := gHP) (L := Addr) (V := MemVal) empty) as (gH) "[inv _]".
-
-      pose (memmap := initMemMap μ).
-      iMod (gen_heap_alloc_big empty memmap (map_disjoint_empty_r memmap) with "inv") as "(inv & res & _)".
-      iModIntro.
-
-      rewrite (right_id empty union memmap).
-
-      iExists (McMemGS gH).
-      iFrame.
-      iExists memmap.
-      iFrame.
-      iPureIntro.
-      apply initMemMap_works.
-    Qed.
-  End RiscvPmpIrisParams.
-
-  Include IrisResources RiscvPmpBase RiscvPmpProgram RiscvPmpSemantics.
-
-End RiscvPmpIrisBase.
-
-Module Import RiscvPmpIrisInstance <:
-  IrisInstance RiscvPmpBase RiscvPmpProgram RiscvPmpSemantics
-    RiscvPmpSignature RiscvPmpIrisBase.
-
-  Section WithSailGS.
-    Import iris.bi.interface.
-    Import iris.bi.big_op.
-    Import iris.base_logic.lib.iprop.
-    Import iris.base_logic.lib.gen_heap.
-    Import Contracts.
-
-    Context `{sailRegGS Σ} `{invGS Σ} `{mG : mcMemGS Σ}.
-
-    Definition reg_file : gset (bv 3) := list_to_set (finite.enum (bv 3)).
-
-    Definition interp_ptsreg `{sailRegGS Σ} (r : RegIdx) (v : Z) : iProp Σ :=
-      match reg_convert r with
-      | Some x => reg_pointsTo x v
-      | None => True
-      end.
-
-    Definition interp_gprs : iProp Σ :=
-      [∗ set] r ∈ reg_file, (∃ v, interp_ptsreg r v)%I.
-
-    Definition PmpEntryCfg : Set := Pmpcfg_ent * Xlenbits.
-
-    Definition interp_pmp_entries (entries : list PmpEntryCfg) : iProp Σ :=
-      match entries with
-      | (cfg0, addr0) :: (cfg1, addr1) :: [] =>
-          reg_pointsTo pmp0cfg cfg0 ∗
-                       reg_pointsTo pmpaddr0 addr0 ∗
-                       reg_pointsTo pmp1cfg cfg1 ∗
-                       reg_pointsTo pmpaddr1 addr1
-      | _ => False
-      end.
-
-    Definition interp_ptsto (addr : Addr) (w : Word) : iProp Σ :=
-      mapsto addr (DfracOwn 1) w.
-    Definition ptstoSth : Addr -> iProp Σ := fun a => (∃ w, interp_ptsto a w)%I.
-    Definition ptstoSthL : list Addr -> iProp Σ :=
-      fun addrs => ([∗ list] k↦a ∈ addrs, ptstoSth a)%I.
-    Lemma ptstoSthL_app {l1 l2} : (ptstoSthL (l1 ++ l2) ⊣⊢ ptstoSthL l1 ∗ ptstoSthL l2)%I.
-    Proof. eapply big_sepL_app. Qed.
-
-    Definition interp_pmp_addr_access (addrs : list Addr) (entries : list PmpEntryCfg) (m : Privilege) : iProp Σ :=
-      [∗ list] a ∈ addrs,
-        (⌜∃ p, Pmp_access a entries m p⌝ -∗ ptstoSth a)%I.
-
-    Definition interp_pmp_addr_access_without (addr : Addr) (addrs : list Addr) (entries : list PmpEntryCfg) (m : Privilege) : iProp Σ :=
-      (ptstoSth addr -∗ interp_pmp_addr_access addrs entries m)%I.
-
-    Definition interp_ptsto_instr (addr : Z) (instr : AST) : iProp Σ :=
-      (∃ v, interp_ptsto addr v ∗ ⌜ pure_decode v = inr instr ⌝)%I.
-
-  End WithSailGS.
-
-  Section RiscvPmpIrisPredicates.
-
-    Definition luser_inst `{sailRegGS Σ, invGS Σ, mcMemGS Σ} (p : Predicate) : Env Val (𝑯_Ty p) -> iProp Σ :=
-      match p return Env Val (𝑯_Ty p) -> iProp Σ with
-      | pmp_entries                   => fun ts => interp_pmp_entries (env.head ts)
-      | pmp_addr_access               => fun ts => interp_pmp_addr_access liveAddrs (env.head (env.tail ts)) (env.head ts)
-      | pmp_addr_access_without       => fun ts => interp_pmp_addr_access_without (env.head (env.tail (env.tail ts))) liveAddrs (env.head (env.tail ts)) (env.head ts)
-      | gprs                          => fun _  => interp_gprs
-      | ptsto                         => fun ts => interp_ptsto (env.head (env.tail ts)) (env.head ts)
-      | encodes_instr                 => fun _ => True%I
-      | ptstomem                      => fun _ => True%I
-      | ptstoinstr                    => fun ts  => interp_ptsto_instr (env.head (env.tail ts)) (env.head ts)%I
-      end.
-
-    Definition lduplicate_inst `{sailRegGS Σ, invGS Σ, mcMemGS Σ} :
-      forall (p : Predicate) (ts : Env Val (𝑯_Ty p)),
-        is_duplicable p = true ->
-        (luser_inst p ts) ⊢ (luser_inst p ts ∗ luser_inst p ts).
-    Proof.
-      iIntros (p ts hdup) "H".
-      destruct p; inversion hdup;
-        iDestruct "H" as "#H";
-        auto.
-    Qed.
-
-  End RiscvPmpIrisPredicates.
-
-  Include IrisSignatureRules RiscvPmpBase RiscvPmpProgram RiscvPmpSemantics
-    RiscvPmpSignature RiscvPmpIrisBase.
-
-End RiscvPmpIrisInstance.
+Import RiscvPmpIrisBase.
+Import RiscvPmpIrisInstance.
 
 Module RiscvPmpModel2.
   Import RiscvPmpSignature.
