case_study/RiscvPmp/IrisInstance.v
@@ -1,0 +1,126 @@
+(******************************************************************************)
+(* Copyright (c) 2020 Steven Keuchel, Dominique Devriese, Sander Huyghebaert  *)
+(* All rights reserved.                                                       *)
+(*                                                                            *)
+(* Redistribution and use in source and binary forms, with or without         *)
+(* modification, are permitted provided that the following conditions are     *)
+(* met:                                                                       *)
+(*                                                                            *)
+(* 1. Redistributions of source code must retain the above copyright notice,  *)
+(*    this list of conditions and the following disclaimer.                   *)
+(*                                                                            *)
+(* 2. Redistributions in binary form must reproduce the above copyright       *)
+(*    notice, this list of conditions and the following disclaimer in the     *)
+(*    documentation and/or other materials provided with the distribution.    *)
+(*                                                                            *)
+(* THIS SOFTWARE IS PROVIDED BY THE COPYRIGHT HOLDERS AND CONTRIBUTORS        *)
+(* "AS IS" AND ANY EXPRESS OR IMPLIED WARRANTIES, INCLUDING, BUT NOT LIMITED  *)
+(* TO, THE IMPLIED WARRANTIES OF MERCHANTABILITY AND FITNESS FOR A PARTICULAR *)
+(* PURPOSE ARE DISCLAIMED. IN NO EVENT SHALL THE COPYRIGHT HOLDER OR          *)
+(* CONTRIBUTORS BE LIABLE FOR ANY DIRECT, INDIRECT, INCIDENTAL, SPECIAL,      *)
+(* EXEMPLARY, OR CONSEQUENTIAL DAMAGES (INCLUDING, BUT NOT LIMITED TO,        *)
+(* PROCUREMENT OF SUBSTITUTE GOODS OR SERVICES; LOSS OF USE, DATA, OR         *)
+(* PROFITS; OR BUSINESS INTERRUPTION) HOWEVER CAUSED AND ON ANY THEORY OF     *)
+(* LIABILITY, WHETHER IN CONTRACT, STRICT LIABILITY, OR TORT (INCLUDING       *)
+(* NEGLIGENCE OR OTHERWISE) ARISING IN ANY WAY OUT OF THE USE OF THIS         *)
+(* SOFTWARE, EVEN IF ADVISED OF THE POSSIBILITY OF SUCH DAMAGE.               *)
+(******************************************************************************)
+
+From Katamaran Require Import
+     Base
+     Iris.Instance
+     Iris.Model
+     Syntax.Predicates
+     RiscvPmp.Base
+     RiscvPmp.Machine
+     RiscvPmp.IrisModel
+     RiscvPmp.Sig.
+
+From iris.base_logic Require Import invariants lib.iprop lib.gen_heap.
+From iris.proofmode Require Import tactics.
+
+Set Implicit Arguments.
+
+Module RiscvPmpIrisInstance <:
+  IrisInstance RiscvPmpBase RiscvPmpProgram RiscvPmpSemantics
+    RiscvPmpSignature RiscvPmpIrisBase.
+  Import RiscvPmpIrisBase.
+  Import RiscvPmpProgram.
+
+  Section WithSailGS.
+    Context `{sailRegGS Σ} `{invGS Σ} `{mG : mcMemGS Σ}.
+
+    Definition reg_file : gset (bv 3) := list_to_set (finite.enum (bv 3)).
+
+    Definition interp_ptsreg `{sailRegGS Σ} (r : RegIdx) (v : Z) : iProp Σ :=
+      match reg_convert r with
+      | Some x => reg_pointsTo x v
+      | None => True
+      end.
+
+    Definition interp_gprs : iProp Σ :=
+      [∗ set] r ∈ reg_file, (∃ v, interp_ptsreg r v)%I.
+
+    Definition PmpEntryCfg : Set := Pmpcfg_ent * Xlenbits.
+
+    Definition interp_pmp_entries (entries : list PmpEntryCfg) : iProp Σ :=
+      match entries with
+      | (cfg0, addr0) :: (cfg1, addr1) :: [] =>
+          reg_pointsTo pmp0cfg cfg0 ∗
+                       reg_pointsTo pmpaddr0 addr0 ∗
+                       reg_pointsTo pmp1cfg cfg1 ∗
+                       reg_pointsTo pmpaddr1 addr1
+      | _ => False
+      end.
+
+    Definition interp_ptsto (addr : Addr) (w : Word) : iProp Σ :=
+      mapsto addr (DfracOwn 1) w.
+    Definition ptstoSth : Addr -> iProp Σ := fun a => (∃ w, interp_ptsto a w)%I.
+    Definition ptstoSthL : list Addr -> iProp Σ :=
+      fun addrs => ([∗ list] k↦a ∈ addrs, ptstoSth a)%I.
+    Lemma ptstoSthL_app {l1 l2} : (ptstoSthL (l1 ++ l2) ⊣⊢ ptstoSthL l1 ∗ ptstoSthL l2)%I.
+    Proof. eapply big_sepL_app. Qed.
+
+    Definition interp_pmp_addr_access (addrs : list Addr) (entries : list PmpEntryCfg) (m : Privilege) : iProp Σ :=
+      [∗ list] a ∈ addrs,
+        (⌜∃ p, Pmp_access a entries m p⌝ -∗ ptstoSth a)%I.
+
+    Definition interp_pmp_addr_access_without (addr : Addr) (addrs : list Addr) (entries : list PmpEntryCfg) (m : Privilege) : iProp Σ :=
+      (ptstoSth addr -∗ interp_pmp_addr_access addrs entries m)%I.
+
+    Definition interp_ptsto_instr (addr : Z) (instr : AST) : iProp Σ :=
+      (∃ v, interp_ptsto addr v ∗ ⌜ pure_decode v = inr instr ⌝)%I.
+
+  End WithSailGS.
+
+  Section RiscvPmpIrisPredicates.
+
+    Definition luser_inst `{sailRegGS Σ, invGS Σ, mcMemGS Σ} (p : Predicate) : Env Val (𝑯_Ty p) -> iProp Σ :=
+      match p return Env Val (𝑯_Ty p) -> iProp Σ with
+      | pmp_entries                   => fun ts => interp_pmp_entries (env.head ts)
+      | pmp_addr_access               => fun ts => interp_pmp_addr_access liveAddrs (env.head (env.tail ts)) (env.head ts)
+      | pmp_addr_access_without       => fun ts => interp_pmp_addr_access_without (env.head (env.tail (env.tail ts))) liveAddrs (env.head (env.tail ts)) (env.head ts)
+      | gprs                          => fun _  => interp_gprs
+      | ptsto                         => fun ts => interp_ptsto (env.head (env.tail ts)) (env.head ts)
+      | encodes_instr                 => fun _ => True%I
+      | ptstomem                      => fun _ => True%I
+      | ptstoinstr                    => fun ts  => interp_ptsto_instr (env.head (env.tail ts)) (env.head ts)%I
+      end.
+
+    Definition lduplicate_inst `{sailRegGS Σ, invGS Σ, mcMemGS Σ} :
+      forall (p : Predicate) (ts : Env Val (𝑯_Ty p)),
+        is_duplicable p = true ->
+        (luser_inst p ts) ⊢ (luser_inst p ts ∗ luser_inst p ts).
+    Proof.
+      iIntros (p ts hdup) "H".
+      destruct p; inversion hdup;
+        iDestruct "H" as "#H";
+        auto.
+    Qed.
+
+  End RiscvPmpIrisPredicates.
+
+  Include IrisSignatureRules RiscvPmpBase RiscvPmpProgram RiscvPmpSemantics
+    RiscvPmpSignature RiscvPmpIrisBase.
+
+End RiscvPmpIrisInstance.
