case_study/RiscvPmp/Machine.v
@@ -33,8 +33,9 @@ From Equations Require Import
      Equations.
 Require Import Equations.Prop.EqDec.
 From Katamaran Require Import
-     Semantics.Registers
      Program
+     Semantics
+     Semantics.Registers
      Syntax.BinOps.
 From Katamaran Require Export
      RiscvPmp.Base.
@@ -1105,3 +1106,6 @@ Module Import RiscvPmpProgram <: Program RiscvPmpBase.
   Include ProgramMixin RiscvPmpBase.
 
 End RiscvPmpProgram.
+
+Module RiscvPmpSemantics <: Semantics RiscvPmpBase RiscvPmpProgram :=
+  MakeSemantics RiscvPmpBase RiscvPmpProgram.
