test/SumMaxLen.v
@@ -43,7 +43,7 @@ From Equations Require Import
      Equations.
 
 From Katamaran Require Import
-     Iris.Logic
+     Iris.Instance
      Iris.Model
      Program
      Semantics
